\documentclass[a4paper,12pt]{article}
\usepackage{mathtools,amsfonts,amssymb,amsmath, bm,commath,multicol}
\usepackage{algorithmicx, tkz-graph, algorithm, fancyhdr, pgfplots}
\usepackage{fancyvrb}

\usepackage[noend]{algpseudocode}



\begin{document}

\section{}

\begin{align*}
Y_t &= e^{at}X_t \\
\frac{d}{dt}Y_t &= ae^{at}X_t + e^{at}\frac{dX_t}{dt} + \frac{1}{2}*0 \\
dY_t &= ae^{at}X_tdt + e^{at}dX_t \\
dY_t &= ae^{at}X_tdt + e^{at}( a(m - X_t)dt + \sigma dB_t) \\
dY_t &= ae^{at}X_tdt + ame^{at}dt - ae^{at}X_tdt + e^{at} \sigma dB_t \\
dY_t &= ame^{at}dt + e^{at} \sigma dB_t \\
\int_o^t dY_sds &= \int_0^t ame^{as}ds + \int_0^t e^{as} \sigma dB_s \\
Y_t - Y_o &= \frac{1}{a} ame^{at} - \frac{1}{a}ame^{a*0} + \int_0^t e^{as} \sigma dB_s \\
e^{at}X_t - X_0 &= me^{at} - me^{0} + \int_0^t e^{as} \sigma dB_s \\
X_t &= X_0e^{-at} + me^{at}e^{-at} - me^{-at} + e^{-at}\sigma \int_0^t e^{as} dB_s \\
X_t &= m - (X_0 - m)e^{-at} + e^{-at}\sigma \int_0^t e^{as} dB_s \\
\end{align*}
o
\section{}
\begin{align*}
\mathbb{E}[X_t] &= \mathbb{E} \bigg[ m - (X_0 - m)e^{-at} + e^{-at}\sigma \int_0^t e^{as} dB_s \bigg] \\
\mathbb{E}[X_t] &= m - (X_0 - m) e^{-at} + e^{-at}\sigma \int_0^t \mathbb{E} \bigg[  e^{as} dB_s \bigg]
\end{align*}



\end{document}